Q1 part 2

BinarySearch-stepwise-refinement.dfy
@@ -3,23 +3,137 @@ predicate Sorted(q: seq<int>)
 	forall i,j :: 0 <= i <= j < |q| ==> q[i] <= q[j] 
 }
 
-method BinarySearch(q: seq<int>, key: int) returns (j: nat)
+predicate Inv(q: seq<int>, key: int, i: nat, j: nat, k: nat)
+{
+	i <= j < k <= |q| 
+	&& key in q[i..k]
+}
+
+
+method {:verify true}BinarySearch(q: seq<int>, key: int) returns (j: nat)
 	requires Sorted(q) && key in q
 	ensures j < |q| && q[j] == key
+{
+	// Introduce local variables + alteration
+	var i: nat, k: nat;
 
-predicate Inv(q: seq<int>, key: int, i: nat, j: nat, k: nat)
+	// assignment 
+	i, j, k := Init(q, key);
+
+	// !Guard ==> q[j] == key  therefore, 
+	// !Guard ==> post
+	j := Iteration(q, key, i, j, k);
+}
+
+
+method Iteration(q: seq<int>, key: int, i0: nat, j0: nat, k0: nat) returns (j: nat)
+	requires Inv(q, key, i0, j0, k0)
+	requires Sorted(q)
+	ensures j <|q|
+	ensures !(Guard1(q, key, j))
+{
+	var i: nat, k : nat;
+	i, j, k := i0, j0, k0;
+	while Guard1(q, key, j)
+		invariant Inv(q, key, i, j, k)
+		decreases V(i, k)
+		{
+			i, j, k := LoopBody(q, key, i, j ,k);
+		}
+
+}
+
+method LoopBody(q: seq<int>, key: int, i0: nat, j0: nat, k0: nat) returns (i :nat, j: nat, k:nat)
+requires Sorted(q)
+requires Inv(q, key, i0, j0, k0)
+requires Guard1(q, key, j0) // q[j0] != key
+ensures Inv(q, key, i, j, k)
+ensures k0 - i0 > k - i 
+ensures j < |q|
+{
+	// Alternate
+	if Guard2(q, key, j0)
+	{
+		updateILemma(q, key, i0, j0, k0);
+		i := UpdateI(q, key, i0, j0, k0);
+		k := k0;
+	}
+	else
+	{
+		updateKLemma(q, key, i0, j0, k0);
+		k := UpdateK(q, key, i0, j0, k0);
+		i := i0;
+	}
+
+	// Assignment
+	j:= (k + i) / 2;
+}
+
 
 predicate method Guard1(q: seq<int>, key: int, j: nat)
+requires 0 <= j < |q|
+{
+	q[j] != key
+}
 
 method Init(q: seq<int>, key: int) returns (i: nat, j: nat, k: nat)
+	requires key in q
+	ensures Inv(q, key, i , j ,k)
+{
+	i := 0;
+	k := |q|; 
+	j := (i + k) / 2;
+}
 
 function V(i: nat, k: nat): int
+{
+	k - i
+}
 
 predicate method Guard2(q: seq<int>, key: int, j: nat)
+requires j < |q|
+{
+	q[j] < key
+}
 
 method UpdateI(q: seq<int>, key: int, i0: nat, j: nat, k: nat) returns (i: nat)
+requires Sorted(q)
+requires j + 1 < k
+requires Inv(q, key, i0, j, k)
+requires q[j] < key
+ensures i > i0
+ensures k > i
+ensures key in q[i..k]
+{
+	i := j + 1;
+}
 
 method UpdateK(q: seq<int>, key: int, i: nat, j: nat, k0: nat) returns (k: nat)
+requires Inv(q, key, i, j, k0)
+requires Sorted(q)
+requires q[j] > key
+requires j > i
+ensures k0 > k > i
+ensures key in q[i..k]
+{
+	k := j;
+}
+
+lemma updateILemma(q: seq<int>, key: int, i: nat, j: nat, k: nat)
+requires Inv(q, key, i, j, k)
+requires q[j] < key
+requires Sorted(q)
+ensures j + 1 < k
+{
+}
+
+lemma updateKLemma(q: seq<int>, key: int, i: nat, j: nat, k: nat)
+requires Inv(q, key, i, j, k)
+requires q[j] > key
+requires Sorted(q)
+ensures i < j
+{
+}
 
 method Main()
 {
